Change name

new-semantics/coq/.CoqMakefile.d
@@ -4,27 +4,27 @@ basics/Basics.vos basics/Basics.vok basics/Basics.required_vos: basics/Basics.v 
 basics/sflib.vo basics/sflib.glob basics/sflib.v.beautified basics/sflib.required_vo: basics/sflib.v 
 basics/sflib.vio: basics/sflib.v 
 basics/sflib.vos basics/sflib.vok basics/sflib.required_vos: basics/sflib.v 
-equivalence/Defs.vo equivalence/Defs.glob equivalence/Defs.v.beautified equivalence/Defs.required_vo: equivalence/Defs.v basics/Basics.vo
-equivalence/Defs.vio: equivalence/Defs.v basics/Basics.vio
-equivalence/Defs.vos equivalence/Defs.vok equivalence/Defs.required_vos: equivalence/Defs.v basics/Basics.vos
-equivalence/EnvSemantics.vo equivalence/EnvSemantics.glob equivalence/EnvSemantics.v.beautified equivalence/EnvSemantics.required_vo: equivalence/EnvSemantics.v basics/Basics.vo equivalence/Defs.vo equivalence/Syntax.vo equivalence/SubstFacts.vo
-equivalence/EnvSemantics.vio: equivalence/EnvSemantics.v basics/Basics.vio equivalence/Defs.vio equivalence/Syntax.vio equivalence/SubstFacts.vio
-equivalence/EnvSemantics.vos equivalence/EnvSemantics.vok equivalence/EnvSemantics.required_vos: equivalence/EnvSemantics.v basics/Basics.vos equivalence/Defs.vos equivalence/Syntax.vos equivalence/SubstFacts.vos
-equivalence/EquivFacts.vo equivalence/EquivFacts.glob equivalence/EquivFacts.v.beautified equivalence/EquivFacts.required_vo: equivalence/EquivFacts.v basics/Basics.vo equivalence/Defs.vo equivalence/SubstFacts.vo
-equivalence/EquivFacts.vio: equivalence/EquivFacts.v basics/Basics.vio equivalence/Defs.vio equivalence/SubstFacts.vio
-equivalence/EquivFacts.vos equivalence/EquivFacts.vok equivalence/EquivFacts.required_vos: equivalence/EquivFacts.v basics/Basics.vos equivalence/Defs.vos equivalence/SubstFacts.vos
-equivalence/MemSemantics.vo equivalence/MemSemantics.glob equivalence/MemSemantics.v.beautified equivalence/MemSemantics.required_vo: equivalence/MemSemantics.v basics/Basics.vo equivalence/Defs.vo equivalence/Syntax.vo equivalence/SubstFacts.vo equivalence/EquivFacts.vo equivalence/EnvSemantics.vo
-equivalence/MemSemantics.vio: equivalence/MemSemantics.v basics/Basics.vio equivalence/Defs.vio equivalence/Syntax.vio equivalence/SubstFacts.vio equivalence/EquivFacts.vio equivalence/EnvSemantics.vio
-equivalence/MemSemantics.vos equivalence/MemSemantics.vok equivalence/MemSemantics.required_vos: equivalence/MemSemantics.v basics/Basics.vos equivalence/Defs.vos equivalence/Syntax.vos equivalence/SubstFacts.vos equivalence/EquivFacts.vos equivalence/EnvSemantics.vos
-equivalence/SubstFacts.vo equivalence/SubstFacts.glob equivalence/SubstFacts.v.beautified equivalence/SubstFacts.required_vo: equivalence/SubstFacts.v basics/Basics.vo equivalence/Defs.vo
-equivalence/SubstFacts.vio: equivalence/SubstFacts.v basics/Basics.vio equivalence/Defs.vio
-equivalence/SubstFacts.vos equivalence/SubstFacts.vok equivalence/SubstFacts.required_vos: equivalence/SubstFacts.v basics/Basics.vos equivalence/Defs.vos
-equivalence/Syntax.vo equivalence/Syntax.glob equivalence/Syntax.v.beautified equivalence/Syntax.required_vo: equivalence/Syntax.v 
-equivalence/Syntax.vio: equivalence/Syntax.v 
-equivalence/Syntax.vos equivalence/Syntax.vok equivalence/Syntax.required_vos: equivalence/Syntax.v 
-equivalence/Typing.vo equivalence/Typing.glob equivalence/Typing.v.beautified equivalence/Typing.required_vo: equivalence/Typing.v basics/Basics.vo equivalence/Defs.vo equivalence/Syntax.vo equivalence/SubstFacts.vo equivalence/EnvSemantics.vo
-equivalence/Typing.vio: equivalence/Typing.v basics/Basics.vio equivalence/Defs.vio equivalence/Syntax.vio equivalence/SubstFacts.vio equivalence/EnvSemantics.vio
-equivalence/Typing.vos equivalence/Typing.vok equivalence/Typing.required_vos: equivalence/Typing.v basics/Basics.vos equivalence/Defs.vos equivalence/Syntax.vos equivalence/SubstFacts.vos equivalence/EnvSemantics.vos
+sim/Defs.vo sim/Defs.glob sim/Defs.v.beautified sim/Defs.required_vo: sim/Defs.v basics/Basics.vo
+sim/Defs.vio: sim/Defs.v basics/Basics.vio
+sim/Defs.vos sim/Defs.vok sim/Defs.required_vos: sim/Defs.v basics/Basics.vos
+sim/EnvSemantics.vo sim/EnvSemantics.glob sim/EnvSemantics.v.beautified sim/EnvSemantics.required_vo: sim/EnvSemantics.v basics/Basics.vo sim/Defs.vo sim/Syntax.vo sim/SubstFacts.vo
+sim/EnvSemantics.vio: sim/EnvSemantics.v basics/Basics.vio sim/Defs.vio sim/Syntax.vio sim/SubstFacts.vio
+sim/EnvSemantics.vos sim/EnvSemantics.vok sim/EnvSemantics.required_vos: sim/EnvSemantics.v basics/Basics.vos sim/Defs.vos sim/Syntax.vos sim/SubstFacts.vos
+sim/MemSemantics.vo sim/MemSemantics.glob sim/MemSemantics.v.beautified sim/MemSemantics.required_vo: sim/MemSemantics.v basics/Basics.vo sim/Defs.vo sim/Syntax.vo sim/SubstFacts.vo sim/SimFacts.vo sim/EnvSemantics.vo
+sim/MemSemantics.vio: sim/MemSemantics.v basics/Basics.vio sim/Defs.vio sim/Syntax.vio sim/SubstFacts.vio sim/SimFacts.vio sim/EnvSemantics.vio
+sim/MemSemantics.vos sim/MemSemantics.vok sim/MemSemantics.required_vos: sim/MemSemantics.v basics/Basics.vos sim/Defs.vos sim/Syntax.vos sim/SubstFacts.vos sim/SimFacts.vos sim/EnvSemantics.vos
+sim/SimFacts.vo sim/SimFacts.glob sim/SimFacts.v.beautified sim/SimFacts.required_vo: sim/SimFacts.v basics/Basics.vo sim/Defs.vo sim/SubstFacts.vo
+sim/SimFacts.vio: sim/SimFacts.v basics/Basics.vio sim/Defs.vio sim/SubstFacts.vio
+sim/SimFacts.vos sim/SimFacts.vok sim/SimFacts.required_vos: sim/SimFacts.v basics/Basics.vos sim/Defs.vos sim/SubstFacts.vos
+sim/SubstFacts.vo sim/SubstFacts.glob sim/SubstFacts.v.beautified sim/SubstFacts.required_vo: sim/SubstFacts.v basics/Basics.vo sim/Defs.vo
+sim/SubstFacts.vio: sim/SubstFacts.v basics/Basics.vio sim/Defs.vio
+sim/SubstFacts.vos sim/SubstFacts.vok sim/SubstFacts.required_vos: sim/SubstFacts.v basics/Basics.vos sim/Defs.vos
+sim/Syntax.vo sim/Syntax.glob sim/Syntax.v.beautified sim/Syntax.required_vo: sim/Syntax.v 
+sim/Syntax.vio: sim/Syntax.v 
+sim/Syntax.vos sim/Syntax.vok sim/Syntax.required_vos: sim/Syntax.v 
+sim/Typing.vo sim/Typing.glob sim/Typing.v.beautified sim/Typing.required_vo: sim/Typing.v basics/Basics.vo sim/Defs.vo sim/Syntax.vo sim/SubstFacts.vo sim/EnvSemantics.vo
+sim/Typing.vio: sim/Typing.v basics/Basics.vio sim/Defs.vio sim/Syntax.vio sim/SubstFacts.vio sim/EnvSemantics.vio
+sim/Typing.vos sim/Typing.vok sim/Typing.required_vos: sim/Typing.v basics/Basics.vos sim/Defs.vos sim/Syntax.vos sim/SubstFacts.vos sim/EnvSemantics.vos
 events/Advance.vo events/Advance.glob events/Advance.v.beautified events/Advance.required_vo: events/Advance.v basics/Basics.vo events/Defs.vo events/Syntax.vo events/SubstFacts.vo events/EnvSemantics.vo events/EquivSemantics.vo events/LinkDefs.vo events/LinkFacts.vo events/EquivLink.vo
 events/Advance.vio: events/Advance.v basics/Basics.vio events/Defs.vio events/Syntax.vio events/SubstFacts.vio events/EnvSemantics.vio events/EquivSemantics.vio events/LinkDefs.vio events/LinkFacts.vio events/EquivLink.vio
 events/Advance.vos events/Advance.vok events/Advance.required_vos: events/Advance.v basics/Basics.vos events/Defs.vos events/Syntax.vos events/SubstFacts.vos events/EnvSemantics.vos events/EquivSemantics.vos events/LinkDefs.vos events/LinkFacts.vos events/EquivLink.vos
