new-semantics/coq/sim/SimFacts.v
@@ -2,12 +2,12 @@ From Basics Require Import Basics.
 From Without_events Require Import Defs.
 From Without_events Require Import SubstFacts.
 
-Section EquivFacts.
+Section SimFacts.
   Variable var : Type.
   Variable loc : Type.
   Variable lang : Type.
 
-  Ltac equiv_lc_tac := 
+  Ltac sim_lc_tac := 
     repeat match goal with
     | _ => solve [auto]
     | H : wvalue (_ _) |- _ => inv H
@@ -17,58 +17,58 @@ Section EquivFacts.
       instantiate (1 := L); ii; exploit H; eauto; ii
     end.
 
-  Lemma equiv_lc_wvl `{Eq loc} (w : wvl var loc lang) :
-    forall f v' m (EQUIV : equiv w f v' m),
+  Lemma sim_lc_wvl `{Eq loc} (w : wvl var loc lang) :
+    forall f v' m (SIM : sim w f v' m),
       wvalue w.
   Proof.
-    ii. induction EQUIV;
+    ii. induction SIM;
     repeat econstructor;
-    equiv_lc_tac.
+    sim_lc_tac.
   Qed.
 
-  Lemma equiv_lc_nv `{Eq loc} :
+  Lemma sim_lc_nv `{Eq loc} :
     forall (σ : nv var loc lang) f v' m
-      (EQUIV : equiv (wvl_v (vl_exp σ)) f v' m),
+      (SIM : sim (wvl_v (vl_exp σ)) f v' m),
     env σ.
-  Proof. ii. eapply equiv_lc_wvl in EQUIV. equiv_lc_tac. Qed.
+  Proof. ii. eapply sim_lc_wvl in SIM. sim_lc_tac. Qed.
 
-  Lemma equiv_lc_vl `{Eq loc} :
+  Lemma sim_lc_vl `{Eq loc} :
     forall (v : vl var loc lang) f v' m
-      (EQUIV : equiv (wvl_v v) f v' m),
+      (SIM : sim (wvl_v v) f v' m),
     value v.
-  Proof. ii. eapply equiv_lc_wvl in EQUIV. equiv_lc_tac. Qed.
+  Proof. ii. eapply sim_lc_wvl in SIM. sim_lc_tac. Qed.
 
-  Lemma equiv_floc_free `{Name loc} (w : wvl var loc lang) f v' m (EQUIV : equiv w f v' m) :
+  Lemma sim_floc_free `{Name loc} (w : wvl var loc lang) f v' m (SIM : sim w f v' m) :
     forall ℓ (FREEw : In ℓ (floc_wvl w)) (FREEf : f ℓ = None),
     m ℓ = None.
   Proof.
-    induction EQUIV; ii; ss; des; clarify; eauto.
+    induction SIM; ii; ss; des; clarify; eauto.
     - rewrite in_app_iff in *; des; eauto.
     - gensym_tac (L ++ floc_vl v) ν.
-      exploit EQUIV; eauto. ii.
+      exploit SIM; eauto. ii.
       match goal with | H : forall _, ~ In _ _ -> _ |- _=> exploit H; eauto end.
       apply open_inc_floc; eauto.
       unfold update. des_goal; eqb2eq loc; clarify.
   Qed.
 
   (* safe for future worlds that preserve free locations *)
-  Lemma equiv_m_ext `{Eq loc} (w : wvl var loc lang) f v' m (EQUIV : equiv w f v' m) :
+  Lemma sim_m_ext `{Eq loc} (w : wvl var loc lang) f v' m (SIM : sim w f v' m) :
     forall m'
       (EXT : forall ℓ, m ℓ <> None -> m' ℓ = m ℓ)
       (AVOID : forall ℓ (FREEw : In ℓ (floc_wvl w)) (FREEf : f ℓ = None), m' ℓ = None),
-    equiv w f v' m'.
+    sim w f v' m'.
   Proof.
-    induction EQUIV; ii; ss.
+    induction SIM; ii; ss.
     - econstructor.
     - econstructor; eauto.
       ii. exploit EXT; eauto. rw. eauto.
-    - eapply equiv_floc; eauto.
+    - eapply sim_floc; eauto.
     - econstructor.
       instantiate (1 := v').
       erewrite EXT; ii; clarify.
-      eapply IHEQUIV1; eauto.
+      eapply IHSIM1; eauto.
       ii. apply AVOID; eauto. rewrite in_app_iff; eauto.
-      eapply IHEQUIV2; eauto.
+      eapply IHSIM2; eauto.
       ii. apply AVOID; eauto. rewrite in_app_iff; eauto.
     - econstructor; eauto.
       instantiate (1 := ℓ').
@@ -84,24 +84,24 @@ Section EquivFacts.
     - econstructor; eauto.
   Qed.
 
-  Lemma equiv_f_ext `{Eq loc} (w : wvl var loc lang) f v' m (EQUIV : equiv w f v' m) :
+  Lemma sim_f_ext `{Eq loc} (w : wvl var loc lang) f v' m (SIM : sim w f v' m) :
     forall f'
       (EXT : forall ℓ (DOM : In ℓ (floc_wvl w)), f ℓ = f' ℓ),
-    equiv w f' v' m.
+    sim w f' v' m.
   Proof.
-    induction EQUIV; ii.
+    induction SIM; ii.
     - econstructor.
     - econstructor; eauto.
       erewrite <- EXT; eauto. s. eauto.
-      eapply IHEQUIV.
+      eapply IHSIM.
       ii. apply EXT; ss; eauto.
-    - eapply equiv_floc; eauto.
+    - eapply sim_floc; eauto.
       erewrite <- EXT; eauto. s. eauto.
-      eapply IHEQUIV.
+      eapply IHSIM.
       ii. apply EXT; ss; eauto.
     - econstructor; eauto.
-      eapply IHEQUIV1. ii. apply EXT; ss; rewrite in_app_iff; eauto.
-      eapply IHEQUIV2. ii. apply EXT; ss; rewrite in_app_iff; eauto.
+      eapply IHSIM1. ii. apply EXT; ss; rewrite in_app_iff; eauto.
+      eapply IHSIM2. ii. apply EXT; ss; rewrite in_app_iff; eauto.
     - econstructor; eauto.
       instantiate (1 := L ++ floc_vl v). ss.
       ii.
@@ -113,18 +113,18 @@ Section EquivFacts.
     - econstructor; eauto.
   Qed.
 
-  Lemma extend_m_floc `{Eq loc} (w : wvl var loc lang) f v' m (EQUIV : equiv w f v' m) :
+  Lemma extend_m_floc `{Eq loc} (w : wvl var loc lang) f v' m (SIM : sim w f v' m) :
     forall ℓ u' (FREEm : m ℓ = None) (FREEf : f ℓ = None),
-      equiv w (ℓ !-> ℓ ; f) v' (ℓ !-> u' ; m).
+      sim w (ℓ !-> ℓ ; f) v' (ℓ !-> u' ; m).
   Proof.
-    induction EQUIV; ii; ss.
+    induction SIM; ii; ss.
     - econstructor.
     - econstructor.
       all: solve [unfold update; des_goal; eqb2eq loc; clarify | eauto].
     - match goal with ℓ : loc, ν : loc |- _ => case_eqb ℓ ν end.
-      + eapply equiv_bloc.
+      + eapply sim_bloc.
         all: solve [unfold update; rewrite eqb_refl; ii; clarify | eauto].
-      + eapply equiv_floc.
+      + eapply sim_floc.
         all: solve [unfold update; des_goal; eqb2eq loc; clarify | eauto].
     - econstructor.
       instantiate (1 := v').
@@ -138,26 +138,26 @@ Section EquivFacts.
       unfold update. des_goal; eqb2eq loc; clarify.
       instantiate (1 := u').
       ii.
-      eapply equiv_f_ext; eauto.
+      eapply sim_f_ext; eauto.
       ii. erewrite update_comm; eauto.
     - econstructor; eauto.
   Qed.
 
-  Lemma reduce_f_bloc `{Name loc} (w : wvl var loc lang) f v' m (EQUIV : equiv w f v' m) :
+  Lemma reduce_f_bloc `{Name loc} (w : wvl var loc lang) f v' m (SIM : sim w f v' m) :
     forall ℓ ℓ' u u'
       (BOUNDf : f ℓ = Some ℓ')
       (BOUNDm : m ℓ' = Some u')
-      (EQUIVu : equiv u (f !! ℓ) u' m),
-    equiv (subst_wvl_wvl u ℓ w) (f !! ℓ) v' m.
+      (SIMu : sim u (f !! ℓ) u' m),
+    sim (subst_wvl_wvl u ℓ w) (f !! ℓ) v' m.
   Proof.
-    induction EQUIV; ii; ss.
+    induction SIM; ii; ss.
     - econstructor.
     - des_goal; eqb2eq loc; clarify.
       + econstructor; eauto.
       + econstructor; eauto.
         unfold remove. des_goal; eqb2eq loc; clarify.
     - des_goal; eqb2eq loc; clarify.
-      eapply equiv_floc; eauto.
+      eapply sim_floc; eauto.
       unfold remove. des_goal; eqb2eq loc; clarify.
     - econstructor; eauto.
     - econstructor; eauto.
@@ -168,32 +168,32 @@ Section EquivFacts.
         exploit (H ν FREE' ℓ _ u); eauto 
       end.
       unfold update. des_goal; eqb2eq loc; clarify.
-      eapply equiv_f_ext; eauto.
+      eapply sim_f_ext; eauto.
       ii. unfold update, remove.
       repeat des_goal; eqb2eq loc; clarify.
       assert (open_loc_subst_wvl_vl _ _ _ v) as RR.
       eapply open_loc_subst_wvl; eauto.
       rewrite RR; eauto.
-      ii. eapply equiv_f_ext; eauto.
+      ii. eapply sim_f_ext; eauto.
       ii. apply remove_update_assoc; eauto.
-      eapply equiv_lc_wvl; eauto.
+      eapply sim_lc_wvl; eauto.
     - econstructor; eauto.
   Qed.
 
-  Lemma equiv_loc_subst `{Eq loc} (w : wvl var loc lang) f v' m (EQUIV : equiv w f v' m) :
+  Lemma sim_loc_subst `{Eq loc} (w : wvl var loc lang) f v' m (SIM : sim w f v' m) :
     forall ℓ ν
       (FRESH : ~ In ν (floc_wvl w))
       (DOMf : f ℓ <> None),
-    equiv (subst_loc_wvl ν ℓ w) (swap f ν ℓ) v' m.
+    sim (subst_loc_wvl ν ℓ w) (swap f ν ℓ) v' m.
   Proof.
-    induction EQUIV; ii; ss;
+    induction SIM; ii; ss;
     try solve [econstructor; eauto].
     - split_nIn. des_goal; eqb2eq loc; clarify.
       + econstructor; eauto. unfold swap. rewrite eqb_refl. auto.
       + econstructor; eauto. unfold swap.
         repeat (des_goal; eqb2eq loc; clarify).
     - split_nIn. des_goal; eqb2eq loc; clarify.
-      eapply equiv_floc; eauto. unfold swap.
+      eapply sim_floc; eauto. unfold swap.
       repeat (des_goal; eqb2eq loc; clarify).
     - rewrite in_app_iff in FRESH. split_nIn.
       econstructor; eauto.
@@ -218,7 +218,7 @@ Section EquivFacts.
       end.
       des; clarify.
       unfold update in *. des_ifs.
-      eapply equiv_f_ext; eauto.
+      eapply sim_f_ext; eauto.
       ii. eapply swap_update_assoc; eauto.
   Qed.
-End EquivFacts.
+End SimFacts.
